Engine/Correctness.v
@@ -80,12 +80,12 @@ Proof.
 Qed.
 
 Theorem pike_vm_to_pike_tree_lazyprefix:
-  forall r lit inp result,
+  forall r inp result,
     pike_regex r -> 
-    trc_pike_vm (compilation r) lit (pike_vm_initial_state_lazyprefix (extract_literal r) inp) (PVS_final result) ->
+    trc_pike_vm (compilation r) (extract_literal r) (pike_vm_initial_state_lazyprefix (extract_literal r) inp) (PVS_final result) ->
     trc_pike_tree (pike_tree_initial_state_lazyprefix rer r inp) (PTS_final result).
 Proof.
-  intros r lit inp result SUBSET TRCVM.
+  intros r inp result SUBSET TRCVM.
   generalize (initial_pike_inv_lazyprefix rer r inp (compilation r) (@eq_refl _ _) SUBSET).
   intros INIT.
   eapply vm_to_tree in TRCVM as [vmfinal [TRCTREE INV]]; eauto.
@@ -131,17 +131,17 @@ Proof.
 Qed.
 
 Theorem pike_vm_correct_lazyprefix:
-  forall r lit inp tree result,
+  forall r inp tree result,
     (* the regex `r` is in the supported subset *)
     pike_regex r ->
     (* `tree` is the tree of the regex `[^]*?r` for the input `inp` *)
     is_tree rer [Areg (lazy_prefix r)] inp GroupMap.empty forward tree ->
     (* the result of the PikeVM is `result` *)
-    trc_pike_vm (compilation r) lit (pike_vm_initial_state_lazyprefix (extract_literal r) inp) (PVS_final result) ->
+    trc_pike_vm (compilation r) (extract_literal r) (pike_vm_initial_state_lazyprefix (extract_literal r) inp) (PVS_final result) ->
     (* This `result` is the priority result of the `tree` *)
     result = first_leaf tree inp.
 Proof.
-  intros r lit inp tree result SUBSET TREE TRC.
+  intros r inp tree result SUBSET TREE TRC.
   eapply encode_equal with (b:=CanExit) in TREE as BOOLTREE; pike_subset.
   eapply pike_vm_to_pike_tree_lazyprefix in TRC; eauto.
   assert (SUBTREE: pike_subtree tree).
